compiler/backend/proofs/source_evalProofScript.sml
@@ -1041,10 +1041,23 @@ Proof
         gvs [s_rel_def, LIST_REL_EL_EQN]
         \\ first_x_assum drule \\ rw []
         \\ Cases_on `EL n refs''` \\ gvs [sv_rel_def]) \\ gvs [] >>
+        gvs[do_opapp_cases, PULL_EXISTS] >>
+        imp_res_tac s_rel_def >> gvs[] >>
+        drule s_rel_clock >> simp[dec_clock_def] >> strip_tac
+      )
+    >- (
+      gvs [oneline dest_thunk_def, AllCaseEqs(), oneline store_lookup_def]
+      \\ `n < LENGTH t''.refs ∧
+          ∃a. EL n t''.refs = Thunk NotEvaluated a ∧
+          v_rel (orac_s t''.eval_state) v a` by (
+        gvs [s_rel_def, LIST_REL_EL_EQN]
+        \\ first_x_assum drule \\ rw []
+        \\ Cases_on `EL n refs''` \\ gvs [sv_rel_def]) \\ gvs [] >>
         gvs[do_opapp_cases, PULL_EXISTS]
         >- (
           imp_res_tac s_rel_def >> gvs[] >>
           drule s_rel_clock >> simp[dec_clock_def] >> strip_tac >>
+          dxrule s_rel_clock >> simp[dec_clock_def] >> strip_tac >>
           last_x_assum dxrule >> simp[] >>
           qmatch_goalsub_abbrev_tac ‘evaluate _ new_env’ >>
           disch_then $ qspec_then ‘new_env’ mp_tac >> impl_tac
@@ -1071,6 +1084,7 @@ Proof
         >- (
           imp_res_tac s_rel_def >> gvs[] >>
           drule s_rel_clock >> simp[dec_clock_def] >> strip_tac >>
+          dxrule s_rel_clock >> simp[dec_clock_def] >> strip_tac >>
           last_x_assum dxrule >> simp[] >>
           qmatch_goalsub_abbrev_tac ‘evaluate _ new_env’ >>
           disch_then $ qspec_then ‘new_env’ mp_tac >> impl_tac
@@ -1109,11 +1123,12 @@ Proof
         gvs [s_rel_def, LIST_REL_EL_EQN]
         \\ first_x_assum drule \\ rw []
         \\ Cases_on `EL n refs''` \\ gvs [sv_rel_def]) \\ gvs [] >>
-        irule_at Any OR_INTRO_THM2 >>
         gvs[do_opapp_cases, PULL_EXISTS]
         >- (
           imp_res_tac s_rel_def >> gvs[] >>
+          irule_at Any OR_INTRO_THM2 >>
           drule s_rel_clock >> simp[dec_clock_def] >> strip_tac >>
+          dxrule s_rel_clock >> simp[dec_clock_def] >> strip_tac >>
           last_x_assum dxrule >> simp[] >>
           qmatch_goalsub_abbrev_tac ‘evaluate _ new_env’ >>
           disch_then $ qspec_then ‘new_env’ mp_tac >> impl_tac
@@ -1122,7 +1137,9 @@ Proof
           )
         >- (
           imp_res_tac s_rel_def >> gvs[] >>
+          irule_at Any OR_INTRO_THM2 >>
           drule s_rel_clock >> simp[dec_clock_def] >> strip_tac >>
+          dxrule s_rel_clock >> simp[dec_clock_def] >> strip_tac >>
           last_x_assum dxrule >> simp[] >>
           qmatch_goalsub_abbrev_tac ‘evaluate _ new_env’ >>
           disch_then $ qspec_then ‘new_env’ mp_tac >> impl_tac
@@ -1772,6 +1789,13 @@ Proof
   DECIDE_TAC
 QED
 
+Triviality less_sub_2_cases:
+  k <= clock /\ ¬(clock ≤ 1) ==>
+  (k = clock \/ k = clock - 1 \/ k <= clock - 2n)
+Proof
+  DECIDE_TAC
+QED
+
 Theorem evaluate_record_suffix:
   (! ^s env exps s' res.
   evaluate s env exps = (s', res) /\
@@ -1841,16 +1865,18 @@ Proof
   \\ simp [combine_dec_result_def]
   >>~ [`getOpClass op = Force`]
   >- (
-    gvs [AllCaseEqs(), dec_clock_def]
-    \\ drule_then (drule_then assume_tac) less_sub_1_cases \\ gvs []
-    \\ imp_res_simp_tac evaluate_is_record_forward \\ gvs [])
+    gvs [AllCaseEqs(), dec_clock_def] >>
+    imp_res_simp_tac evaluate_is_record_forward >> gvs []
+    >- simp[record_forward_refl]
+    >- simp[DISJ_EQ_IMP, record_forward_refl] >>
+    drule_then (drule_then assume_tac) less_sub_2_cases >> gvs []
+    )
   >- (
     gvs [AllCaseEqs(), dec_clock_def]
     \\ imp_res_simp_tac evaluate_is_record_forward \\ gvs []
     >- (drule_then irule record_forward_trans \\ gvs [])
     >- (drule_then irule record_forward_trans \\ gvs [])
     >- (disj2_tac \\ drule_then irule record_forward_trans \\ gvs []))
-  \\ gs[]
 QED
 
 (* Constructs the oracle from an evaluation by using the recorded
